lawyer/nonblocking/tokens/om_wfree_inst_tokens.v
@@ -1,0 +1,68 @@
+From iris.proofmode Require Import tactics.
+From lawyer.examples Require Import orders_lib.
+From lawyer.obligations Require Import env_helpers obligations_model.
+From lawyer.nonblocking Require Import om_wfree_inst.
+From lawyer.nonblocking.logrel Require Import logrel.
+
+
+From trillium.program_logic Require Import weakestpre. 
+From heap_lang Require Import heap_lang_defs lang notation.
+From lawyer.obligations Require Import obligations_resources.
+
+
+Lemma foo:
+  forall {M: Model} {EM: ExecutionModel heap_lang M} {Σ} {OHE: OM_HL_Env OP_HL_WF EM Σ},
+    heap1GS Σ.
+Proof using.
+  intros.
+  exact (iem_phys _ EM).
+  Show Proof.
+  Abort. 
+
+Lemma foo:
+  forall {M: Model} {EM: ExecutionModel heap_lang M} {Σ} {OHE: OM_HL_Env OP_HL_WF EM Σ},
+    invGS_gen HasNoLc Σ.
+Proof using.
+  intros.
+  apply _.
+  Show Proof. 
+Abort. 
+
+
+(* TODO: generalize the token type *)
+From iris.algebra Require Import excl. 
+Class UnitTokenPre Σ := {
+    ut_pre_tok :: inG Σ (exclR unit);
+}.
+Class UnitToken Σ := {
+    ut_pre_pre :: UnitTokenPre Σ;
+    ut_γ: gname;
+}.
+Definition unit_tok `{UnitToken Σ} := own ut_γ (Excl ()). 
+
+Record WaitFreeSpecToken (m: val) := {
+  wfst_is_init_st: cfg heap_lang -> Prop;
+  (** for wait-free modules, we expect that invariant doesn't contain OM resources *)
+  wfst_mod_inv {Σ} {hG: heap1GS Σ} {iG: invGS_gen HasNoLc Σ}: iProp Σ;
+  wfst_mod_inv_Pers `{heap1GS Σ, invGS_gen HasNoLc Σ} ::
+    Persistent wfst_mod_inv;
+  wfst_init_mod `{heap1GS Σ, invGS_gen HasNoLc Σ}:
+    forall c (INIT: wfst_is_init_st c),
+      ⊢ hl_phys_init_resource c ={⊤}=∗ wfst_mod_inv;
+  wfst_F: nat;
+  wfst_spec:
+  forall {M: Model} {EM: ExecutionModel heap_lang M} {Σ} {OHE: OM_HL_Env OP_HL_WF EM Σ}
+    {UT: UnitToken Σ}
+    τ π q (a: val),
+    {{{ cp_mul π d_wfr0 wfst_F ∗ th_phase_frag τ π q ∗ 
+        (let _: heap1GS Σ := iem_phys HeapLangEM EM in wfst_mod_inv ) ∗
+        unit_tok
+    }}}
+      App m a @ τ
+    {{{ v, RET v; th_phase_frag τ π q ∗ unit_tok}}};
+
+  (* (* TODO: derive it from wfs_spec *) *)
+  (* wfs_safety_spec: *)
+  (*   ∀ {Σ : gFunctors} `{heap1GS Σ, invGS_gen HasNoLc Σ}, *)
+  (*     wfs_mod_inv ⊢ interp m; *)
+}. 
